src/Crypto/Digests.dfy
@@ -7,7 +7,7 @@ module {:extern "Digests"} Digests {
   datatype {:extern "KEY_DERIVATION_ALGORITHM"} KEY_DERIVATION_ALGORITHM = HKDF_WITH_SHA_384 | HKDF_WITH_SHA_256 | IDENTITY
 
   // Hash length in octets (bytes), e.g. HashLength(SHA256) = 256 = 32 * 8
-  function HashLength(algorithm: KEY_DERIVATION_ALGORITHM): (n: nat)
+  function HashLength(algorithm: KEY_DERIVATION_ALGORITHM): (n: int32)
     ensures algorithm == HKDF_WITH_SHA_256 ==> n == 32
     ensures algorithm == HKDF_WITH_SHA_384 ==> n == 48
     ensures algorithm == IDENTITY ==> n == 0
@@ -20,5 +20,5 @@ module {:extern "Digests"} Digests {
   }
 
     function {:axiom} Hash(algorithm: KEY_DERIVATION_ALGORITHM, key: seq<uint8>, message: seq<uint8>): (s: seq<uint8>)
-      ensures |s| == HashLength(algorithm)
+      ensures |s| == HashLength(algorithm) as int
 }
