src/Crypto/HKDF/HKDFSpec.dfy
@@ -9,7 +9,7 @@ module HKDFSpec {
   // return T(i)
   function Ti(algorithm: KEY_DERIVATION_ALGORITHM, key: seq<uint8>, info: seq<uint8>, i: nat): seq<uint8>
     requires 0 <= i < 256
-    requires HashLength(algorithm) <= |key|
+    requires HashLength(algorithm) as int <= |key|
     decreases i, 1
   {
     if i == 0 then [] else
@@ -19,7 +19,7 @@ module HKDFSpec {
   // return T(i-1) | info | i
   function PreTi(algorithm: KEY_DERIVATION_ALGORITHM, key: seq<uint8>, info: seq<uint8>, i: nat): seq<uint8>
     requires 1 <= i < 256
-    requires HashLength(algorithm) <= |key|
+    requires HashLength(algorithm) as int <= |key|
     decreases i, 0
   {
     Ti(algorithm, key, info, i-1) + info + [(i as uint8)]
@@ -28,7 +28,7 @@ module HKDFSpec {
   // return T(1) | T(2) | ... | T(n)
   function T(algorithm: KEY_DERIVATION_ALGORITHM, key: seq<uint8>, info: seq<uint8>, n: nat): seq<uint8>
     requires 0 <= n < 256
-    requires HashLength(algorithm) <= |key|
+    requires HashLength(algorithm) as int <= |key|
     decreases n
   {
     if n == 0 then [] else
@@ -37,14 +37,14 @@ module HKDFSpec {
 
   lemma TLength(algorithm: KEY_DERIVATION_ALGORITHM, key: seq<uint8>, info: seq<uint8>, n: nat)
     requires 0 <= n < 256
-    requires HashLength(algorithm) <= |key|
-    ensures |T(algorithm, key, info, n)| == n * HashLength(algorithm)
+    requires HashLength(algorithm) as int <= |key|
+    ensures |T(algorithm, key, info, n)| == n * HashLength(algorithm) as int
   {
   }
 
   lemma TPrefix(algorithm: KEY_DERIVATION_ALGORITHM, key: seq<uint8>, info: seq<uint8>, m: nat, n: nat)
     requires 0 <= m <= n < 256
-    requires HashLength(algorithm) <= |key|
+    requires HashLength(algorithm) as int <= |key|
     ensures T(algorithm, key, info, m) <= T(algorithm, key, info, n)
   {
     if m == n {
@@ -54,8 +54,8 @@ module HKDFSpec {
   }
 
   function TMaxLength(algorithm: KEY_DERIVATION_ALGORITHM, key: seq<uint8>, info: seq<uint8>): (result: seq<uint8>)
-    requires HashLength(algorithm) <= |key|
-    ensures |result| == 255 * HashLength(algorithm)
+    requires HashLength(algorithm) as int <= |key|
+    ensures |result| == 255 * HashLength(algorithm) as int
   {
     TLength(algorithm, key, info, 255);
     T(algorithm, key, info, 255)
